cputnewC

monad_model.v
@@ -1666,17 +1666,17 @@ Definition locT_nat := [eqType of nat].
 Module ModelTypedStore.
 
 Section ModelTypedStore.
-Variables (ml_type0' : eqType) (coq_type0 : ml_type0' -> Type)
-          (ml_nonempty0 : ml_type0') (val_nonempty0 : coq_type0 ml_nonempty0).
+Variables (ml_type0 : eqType) (coq_type0 : ml_type0 -> Type)
+          (ml_nonempty0 : ml_type0) (val_nonempty0 : coq_type0 ml_nonempty0).
 
-Definition ml_type0 : Type := ml_type0'.
+Definition ml_type : Type := ml_type0.
 
-HB.instance Definition _ := @isML_universe.Build ml_type0
-  (Equality.class ml_type0') (fun M => @coq_type0) ml_nonempty0
+HB.instance Definition _ := @isML_universe.Build ml_type
+  (Equality.class ml_type0) (fun M => @coq_type0) ml_nonempty0
   (fun M => val_nonempty0).
 
 Record binding (M : Type -> Type) :=
-  mkbind { bind_type : ml_type0; bind_val : coq_type M bind_type }.
+  mkbind { bind_type : ml_type; bind_val : coq_type M bind_type }.
 
 Arguments mkbind {M}.
 
@@ -1684,13 +1684,13 @@ Definition acto : UU0 -> UU0 :=
   MS (seq (binding idfun)) [the monad of option_monad].
 Local Notation M := acto.
 
-Local Notation coq_type' := (@coq_type ml_type0 idfun).
+Local Notation coq_type' := (@coq_type ml_type idfun).
 
 Definition def : binding idfun := mkbind ml_nonempty (val_nonempty idfun).
 
 Local Notation nth_error := List.nth_error.
 
-Notation loc := (@loc ml_type0 locT_nat).
+Notation loc := (@loc ml_type locT_nat).
 
 Definition cnew T (v : coq_type M T) : M (loc T) :=
   fun st => let n := size st in
@@ -1719,7 +1719,7 @@ Definition crun (A : UU0) (m : M A) : option A :=
 
 Definition Env := seq (binding idfun).
 
-Definition fresh_loc (T : ml_type0) (e : Env) := mkloc T (size e).
+Definition fresh_loc (T : ml_type) (e : Env) := mkloc T (size e).
 
 Section mkbind.
 Local Notation mkbind := (@mkbind idfun).
@@ -1727,7 +1727,7 @@ Local Notation mkbind := (@mkbind idfun).
 Definition extend_env T (v : coq_type M T) (e : Env) :=
   rcons e (mkbind T v).
 
-Variant nth_error_spec (T : ml_type0) (e : Env) (r : loc T) : Type :=
+Variant nth_error_spec (T : ml_type) (e : Env) (r : loc T) : Type :=
   | NthError : forall s : coq_type M T,
     nth_error e (loc_id r) = Some (mkbind T s) -> nth_error_spec e r
   | NthError_nocoerce : forall T' (s' : coq_type M T'),
@@ -1735,7 +1735,7 @@ Variant nth_error_spec (T : ml_type0) (e : Env) (r : loc T) : Type :=
     nth_error_spec e r
   | NthError_None : nth_error e (loc_id r) = None -> nth_error_spec e r.
 
-Lemma ntherrorP (T : ml_type0) (e : Env) (r : loc T) : nth_error_spec e r.
+Lemma ntherrorP (T : ml_type) (e : Env) (r : loc T) : nth_error_spec e r.
 Proof.
 case H : (nth_error e (loc_id r)) => [[T' s']|].
   have [Ts'|Ts'] := boolp.pselect (coerce T s').
@@ -1776,7 +1776,8 @@ Lemma nocoerce_cget T (r : loc T) T' (s' : coq_type M T') e :
   cget r e = fail.
 Proof. by move=> H Ts'; rewrite /cget H; case: coerce Ts'. Qed.
 
-Lemma nocoerce_cput T (r : loc T) (s : coq_type M T) (T' : ml_type0) (s' : coq_type M T') e :
+Lemma nocoerce_cput T (r : loc T) (s : coq_type M T) (T' : ml_type)
+    (s' : coq_type M T') e :
   nth_error e (loc_id r) = Some (mkbind T' s') ->
   ~ coerce T s' ->
   cput r s e = fail.
@@ -1858,7 +1859,7 @@ have [s' H|T' s' H Ts'|H] := ntherrorP e r.
 - by rewrite 2!MS_bindE None_cput.
 Qed.
 
-Lemma Some_cputput (T : ml_type0) (r : loc T) (s s' : coq_type M T)
+Lemma Some_cputput (T : ml_type) (r : loc T) (s s' : coq_type M T)
   (e : Env) (s'' : coq_type M T) :
   nth_error e (loc_id r) = Some (mkbind T s'') ->
   (cput r s >> cput r s') e = cput r s' e.
@@ -2093,21 +2094,15 @@ Lemma cputnewC T T' (r : loc T) (s : coq_type M T) (s' : coq_type M T') A
   cput r s >> (cnew s' >>= k).
 Proof.
 apply/boolp.funext => e /=.
-rewrite bindE /= /bindS MS_mapE /= fmapE /= bindA /=.
-rewrite [in RHS]bindE /= /bindS MS_mapE /= fmapE /= bindA /= /cget /cput.
-case Hr: (nth_error _ _) => [[T1 u]|]; last by rewrite bindfailf.
-case: (eqVneq T1 T) => H //=; last by rewrite coerce_None// 1?eq_sym// coerce_None// eq_sym.
-subst T1.
-rewrite [in LHS]coerce_Some//.
-rewrite bindE /= /bindS /= bindE /= bindE /= /bindS /= MS_mapE /= fmapE /=.
-rewrite bindE /= /bindS /= bindE /= bindE /= /bindS /= MS_mapE /= fmapE /=.
-rewrite (nth_error_rcons_some _ Hr).
-rewrite coerce_Some.
-rewrite bindE /= /bindS /= bindE /= bindE /= /bindS /= MS_mapE /= fmapE /=.
-rewrite bindE /= /bindS /=.
-rewrite /fresh_loc/=.
-rewrite (nth_error_size_set_nth _ _ Hr).
-by rewrite (nth_error_set_nth_rcons _ _ _ Hr).
+have [u Hr|T1 s1' Hr T1s'|Hr] := ntherrorP e r.
+- rewrite (Some_cget _ _ _ _ Hr).
+  rewrite [RHS]MS_bindE [in RHS]/cput Hr coerce_Some bindretf/=.
+  rewrite !MS_bindE /cnew !bindretf/= !MS_bindE /cput.
+  rewrite (nth_error_rcons_some _ Hr) coerce_Some bindretf/=.
+  by rewrite (nth_error_size_set_nth _ _ Hr) (nth_error_set_nth_rcons _ _ _ Hr).
+- rewrite 2!MS_bindE (nocoerce_cget _ T1s')// bindfailf.
+  by rewrite (nocoerce_cput _ _ T1s').
+- by rewrite 2!MS_bindE None_cget// bindfailf None_cput.
 Qed.
 
 Definition crunret (A B : UU0) (m : M A) (s : B) :
@@ -2161,7 +2156,7 @@ Qed.
 
 HB.instance Definition _ := Monad.on M.
 HB.instance Definition isMonadTypedStoreModel :=
-  isMonadTypedStore.Build ml_type0 locT_nat M cnewget cnewput cgetput cgetputskip
+  isMonadTypedStore.Build ml_type locT_nat M cnewget cnewput cgetput cgetputskip
     cgetget cputget cputput cgetC cgetnewD cgetnewE cgetputC cputC
     cputgetC cputnewC
     crunret crunskip crunnew crunnewget crungetnew crungetput.
